new/golang/theory/mem.v
@@ -10,594 +10,100 @@ Set Default Proof Mode "Classic".
 Set Default Proof Using "Type".
 
 Section goose_lang.
-  Context `{ffi_sem: ffi_semantics} `{!ffi_interp ffi} `{!heapGS Σ}.
 
-  Context `{!IntoVal V}.
-  Context `{!IntoValTyped V t}.
-  Implicit Type v : V.
-  Program Definition typed_pointsto_def l (dq : dfrac) (v : V) : iProp Σ :=
-    (([∗ list] j↦vj ∈ flatten_struct (to_val v), heap_pointsto (l +ₗ j) dq vj))%I.
-  Definition typed_pointsto_aux : seal (@typed_pointsto_def). Proof. by eexists. Qed.
-  Definition typed_pointsto := typed_pointsto_aux.(unseal).
-  Definition typed_pointsto_unseal : @typed_pointsto = @typed_pointsto_def := typed_pointsto_aux.(seal_eq).
+  Context `{sem: ffi_semantics} `{!ffi_interp ffi} `{!heapGS Σ}.
 
-  Notation "l ↦ dq v" := (typed_pointsto l dq v%V)
-                                   (at level 20, dq custom dfrac at level 1,
-                                    format "l  ↦ dq  v") : bi_scope.
+  Inductive is_cmpxchg_type : ∀ (t : go.type) (V : Type) `{!IntoVal V} `{!TypedPointsto V}, Prop :=
+  | is_cmpxchg_type_uint64 : is_cmpxchg_type go.uint64 w64
+  | is_cmpxchg_type_uint32 : is_cmpxchg_type go.uint32 w32
+  | is_cmpxchg_type_uint16 : is_cmpxchg_type go.uint16 w16
+  | is_cmpxchg_type_uint8 : is_cmpxchg_type go.uint8 w8
+  | is_cmpxchg_type_int64 : is_cmpxchg_type go.int64 w64
+  | is_cmpxchg_type_int32 : is_cmpxchg_type go.int32 w32
+  | is_cmpxchg_type_int16 : is_cmpxchg_type go.int16 w16
+  | is_cmpxchg_type_int8 : is_cmpxchg_type go.int8 w8
+  | is_cmpxchg_type_bool : is_cmpxchg_type go.bool bool.
 
-  Ltac unseal := rewrite ?typed_pointsto_unseal /typed_pointsto_def.
-
-  Global Instance typed_pointsto_timeless l q v : Timeless (l ↦{q} v).
-  Proof. unseal. apply _. Qed.
-
-  Global Instance typed_pointsto_persistent l v : Persistent (l ↦□ v).
-  Proof. unseal. apply _. Qed.
-
-  Global Instance typed_pointsto_dfractional l v : DFractional (λ dq, l ↦{dq} v)%I.
-  Proof. unseal. apply _. Qed.
-  Global Instance typed_pointsto_as_dfractional l v dq : AsDFractional
-                                                     (l ↦{dq} v)
-                                                     (λ dq, l ↦{dq} v)%I dq.
-  Proof. auto. Qed.
-
-  Global Instance typed_pointsto_fractional l v : Fractional (λ q, l ↦{#q} v)%I.
-  Proof. unseal. apply _. Qed.
-
-  Global Instance typed_pointsto_as_fractional l v q : AsFractional
-                                                     (l ↦{#q} v)
-                                                     (λ q, l ↦{#q} v)%I q.
-  Proof. auto. Qed.
-
-  Lemma alist_val_inj a b :
-    alist_val a = alist_val b →
-    a = b.
-  Proof.
-    rewrite alist_val_unseal.
-    dependent induction b generalizing a.
-    { by destruct a as [|[]]. }
-    destruct a0.
-    destruct a as [|[]]; first done.
-    rewrite /= => [=].
-    intros. subst.
-    repeat f_equal.
-    - by apply to_val_inj.
-    - by apply IHb.
-  Qed.
-
-  Local Lemma flatten_struct_inj (v1 v2 : val) :
-    has_go_type v1 t → has_go_type v2 t →
-    flatten_struct v1 = flatten_struct v2 → v1 = v2.
-  Proof.
-    intros Hty1 Hty2 Heq.
-    clear dependent V.
-    dependent induction Hty1 generalizing v2.
-    Ltac2 step () :=
-      match! goal with
-      | [ v : slice.t |- _ ] => let v := Control.hyp v in destruct $v
-      | [ v : interface.t |- _ ] => let v := Control.hyp v in destruct $v
-      (* | [ v : interface.tSome |- _ ] => let v := Control.hyp v in destruct $v *)
-      | [ v : func.t |- _ ] => let v := Control.hyp v in destruct $v
-      | [ v : option (go_string * go_string )|- _ ] => let v := Control.hyp v in destruct $v as [[??]|]
-      | [ h : has_go_type _ _ |- _ ] => let h := Control.hyp h in (inversion_clear $h in Heq)
-      | [ h : alist_val _ = alist_val _ |- _ ] => apply alist_val_inj in $h; subst
-
-      (* unseal whatever's relevant *)
-      | [ h : context [struct.val_aux]  |- _ ] => rewrite !struct.val_aux_unseal in $h
-      | [ |- context [struct.val_aux] ] => rewrite !struct.val_aux_unseal
-      | [ h : context [to_val]  |- _ ] => rewrite !to_val_unseal in $h
-      | [ |- context [to_val] ] => rewrite !to_val_unseal
-
-      | [ h : (flatten_struct _ = flatten_struct _) |- _ ] => progress (simpl in $h)
-      | [ h : cons _ _ = cons _ _  |- _ ] =>
-          Std.inversion Std.FullInversion (Std.ElimOnIdent h) None None;
-          clear $h; subst
-      | [ h : context [length (cons _ _)] |- _ ] => progress (simpl in $h)
-      | [ h : context [length []] |- _ ] => progress (simpl in $h)
-      | [ |- _ ] => reflexivity
-      | [ |- _ ] => discriminate
-      end
-    .
-    all: repeat ltac2:(step ()).
-    {
-      (* XXX: need to reorder hyps to avoid an error in [dependent induction].... *)
-      move a after a0. subst.
-      dependent induction a generalizing a0.
-      { destruct a0; done. }
-      dependent destruction a0; first done.
-      simpl in Heq.
-      apply app_inj_1 in Heq as [? ?].
-      2:{ by do 2 erewrite has_go_type_len by naive_solver. }
-      simpl. f_equal.
-      + apply H; naive_solver.
-      + apply IHa; naive_solver.
-    }
-    {
-      induction d as [|[]d]; repeat ltac2:(step ()).
-      simpl in *.
-      apply app_inj_1 in Heq as [? ?].
-      2:{ by do 2 erewrite has_go_type_len by naive_solver. }
-      f_equal.
-      + apply H; naive_solver.
-      + apply IHd; naive_solver.
-    }
-  Qed.
-
-  Lemma typed_pointsto_zero_size l dq v :
-    go_type_size t = 0%nat →
-    ⊢ l ↦{dq} v.
-  Proof using IntoValTyped0.
-    unseal.
-    intros Hz.
-    pose proof (to_val_has_go_type (V:=V) v) as Hlen%has_go_type_len.
-    rewrite Hz in Hlen.
-    apply length_zero_iff_nil in Hlen.
-    rewrite Hlen /=.
-    auto.
-  Qed.
-
-  Lemma typed_pointsto_valid l dq v :
-    l ↦{dq} v ⊢ ⌜go_type_size t > 0 → ✓dq⌝.
-  Proof using IntoValTyped0.
-    iIntros "H".
-    unseal.
-    pose proof (to_val_has_go_type v) as H.
-    destruct (flatten_struct (#v)) eqn:Hbad.
-    { apply (f_equal length) in Hbad. rewrite (has_go_type_len (t:=t)) //= in Hbad.
-      iPureIntro. lia. }
-    iDestruct "H" as "[H1 H2]".
-    iDestruct (heap_pointsto_valid with "H1") as %Hvalid; done.
-  Qed.
-
-  Global Instance typed_pointsto_combine_sep_gives l dq1 dq2 v1 v2 :
-    CombineSepGives (l ↦{dq1} v1)%I (l ↦{dq2} v2)%I
-                    ⌜ (go_type_size t > O → ✓(dq1 ⋅ dq2)) ∧ v1 = v2 ⌝%I.
-  Proof using IntoValTyped0.
-    unfold CombineSepGives.
-    unseal.
-    iIntros "[H1 H2]".
-    rename l into l'.
-    pose proof (to_val_has_go_type v1) as H1.
-    pose proof (to_val_has_go_type v2) as H2.
-    pose proof (flatten_struct_inj _ _ H1 H2).
-    iDestruct (big_sepL2_sepL_2 with "H1 H2") as "H".
-    { do 2 (erewrite has_go_type_len by done). done. }
-    iDestruct (big_sepL2_impl with "H []") as "H".
-    {
-      iModIntro. iIntros "*%%[H1 H2]".
-      iCombine "H1 H2" gives %Heq.
-      instantiate(1:=(λ _ _ _, ⌜ _ ⌝%I )).
-      simpl. iPureIntro. exact Heq.
-    }
-    iDestruct (big_sepL2_pure with "H") as %[Hlen Heq].
-    iModIntro. iPureIntro.
-    split.
-    { intros. specialize (Heq 0%nat).
-      destruct (flatten_struct (# v1)) eqn:Hbad.
-      { exfalso. apply (f_equal length) in Hbad. rewrite (has_go_type_len (t:=t)) /= in Hbad; [lia|done]. }
-      clear Hbad.
-      destruct (flatten_struct (# v2)) eqn:Hbad.
-      { exfalso. apply (f_equal length) in Hbad. rewrite (has_go_type_len (t:=t)) /= in Hbad; [lia|done]. }
-      specialize (Heq v v0 ltac:(done) ltac:(done)) as [??]. assumption.
-    }
-    {
-      apply to_val_inj, H.
-      apply list_eq.
-      intros.
-      replace i with (i + 0)%nat by lia.
-      rewrite <- !lookup_drop.
-      destruct (drop i $ flatten_struct (# v1)) eqn:Hlen1, (drop i $ flatten_struct (# v2)) eqn:Hlen2.
-      { done. }
-      1-2: exfalso; apply (f_equal length) in Hlen1, Hlen2;
-        rewrite !length_drop in Hlen1, Hlen2;
-        simpl in *; lia.
-      specialize (Heq i v v0).
-      replace i with (i + 0)%nat in Heq by lia.
-      rewrite <- !lookup_drop in Heq.
-      rewrite Hlen1 Hlen2 in Heq.
-      simpl in Heq.
-      unshelve epose proof (Heq _ _); naive_solver.
-    }
-  Qed.
-
-  Lemma typed_pointsto_persist l dq v :
-    l ↦{dq} v ==∗ l ↦□ v.
-  Proof.
-    iIntros "H". iPersist "H". done.
-  Qed.
-
-  #[global]
-  Instance typed_pointsto_update_persist l dq v :
-    UpdateIntoPersistently (l ↦{dq} v) (l ↦□ v).
-  Proof. apply _. Qed.
-
-  Lemma typed_pointsto_not_null l dq v :
-    go_type_size t > 0 →
-    l ↦{dq} v -∗ ⌜ l ≠ null ⌝.
-  Proof using IntoValTyped0.
-    unseal. intros Hlen. iIntros "?".
-    pose proof (to_val_has_go_type v) as Hty.
-    generalize dependent (# v). clear dependent V. intros v Hty.
-    iInduction Hty as [] "IH"; subst;
-    simpl; rewrite ?to_val_unseal /= ?right_id ?loc_add_0;
-      try (iApply heap_pointsto_non_null; by iFrame).
-    - (* interface *)
-      destruct i;
-        simpl; rewrite ?to_val_unseal /= ?right_id ?loc_add_0;
-        try (iApply heap_pointsto_non_null; by iFrame).
-    - (* array *)
-      rewrite go_type_size_unseal /= in Hlen.
-      destruct a as [|].
-      { exfalso. simpl in *. lia. }
-      destruct (decide (go_type_size_def elem = O)).
-      { exfalso. rewrite e in Hlen. simpl in *. lia. }
-      iDestruct select ([∗ list] _ ↦ _ ∈ _, _)%I as "[? _]".
-      iApply ("IH" $! v with "").
-      + naive_solver.
-      + iPureIntro. rewrite go_type_size_unseal. lia.
-      + iFrame.
-    - (* struct *)
-      rewrite go_type_size_unseal /= in Hlen.
-      iInduction d as [|[a]] "IH2"; simpl in *.
-      { exfalso. lia. }
-      rewrite struct.val_aux_unseal /=.
-      destruct (decide (go_type_size_def g = O)).
-      {
-        rewrite (nil_length_inv (flatten_struct (default _ _))).
-        2:{
-          erewrite has_go_type_len.
-          { rewrite go_type_size_unseal. done. }
-          apply Hfields. by left.
-        }
-        rewrite app_nil_l.
-        iApply ("IH2" with "[] [] [] [$]").
-        - iPureIntro. intros. apply Hfields. by right.
-        - iPureIntro. lia.
-        - iModIntro. iIntros. iApply ("IH" with "[] [] [$]").
-          + iPureIntro. by right.
-          + iPureIntro. lia.
-      }
-      {
-        iDestruct select ([∗ list] _ ↦ _ ∈ _, _)%I as "[? _]".
-        iApply ("IH" with "[] [] [$]").
-        - iPureIntro. by left.
-        - iPureIntro. rewrite go_type_size_unseal. lia.
-      }
-  Qed.
-
-  Lemma wp_alloc stk E :
-    {{{ True }}}
-      mem.alloc t (#()) @ stk; E
-    {{{ l, RET #l; l ↦ (default_val V) }}}.
-  Proof.
-    iIntros (Φ) "_ HΦ".
-    rewrite mem.alloc_unseal.
-    wp_call.
-    iApply (wp_allocN_seq with "[//]"); first by word. iNext.
-    change (uint.nat 1) with 1%nat; simpl.
-    iIntros (l) "[Hl _]".
-    rewrite to_val_unseal /= -to_val_unseal.
-    iApply "HΦ".
-    unseal.
-    rewrite Z.mul_0_r loc_add_0.
-    iFrame.
-  Qed.
-
-  Lemma wp_mem_load stk E q l v :
-    {{{ ▷ l ↦{q} v }}}
-      ![t] #l @ stk; E
-    {{{ RET #v; l ↦{q} v }}}.
-  Proof using IntoValTyped0.
-    iIntros (Φ) ">Hl HΦ".
-    unseal.
-    pose proof (to_val_has_go_type v) as Hty.
-    generalize dependent (# v). clear dependent V.
-    intros v Hty.
-    iAssert (▷ (([∗ list] j↦vj ∈ flatten_struct v, heap_pointsto (l +ₗ j) q vj) -∗ Φ v))%I with "[HΦ]" as "HΦ".
-    { iIntros "!> HPost".
-      iApply "HΦ". iFrame. }
-    rewrite mem.load_unseal.
-    rename l into l'.
-    iInduction Hty as [] "IH" forall (l' Φ) "HΦ".
-    all: try destruct i.
-    all: rewrite ?to_val_unseal /= /= ?loc_add_0 ?right_id; wp_pures.
-    all: try (iApply (wp_load with "[$]"); done).
-    - (* case arrayT *)
-      subst.
-      iInduction a as [|] "IH2" forall (l' Φ).
-      { simpl. wp_pures. rewrite to_val_unseal. iApply "HΦ". by iFrame. }
-      wp_pures.
-      iDestruct "Hl" as "[Hf Hl]".
-      fold flatten_struct.
-      simpl. wp_pures.
-      simpl.
-      wp_apply ("IH" with "[] Hf").
-      { iPureIntro. by left. }
-      iIntros "Hf".
-      wp_pures.
-      replace (LitV (LitLoc l')) with (# l').
-      2:{ by rewrite to_val_unseal. }
-      wp_pures.
-      rewrite to_val_unseal /=.
-      wp_apply ("IH2" with "[] [] [Hl]").
-      { iPureIntro. intros. apply Helems. by right. }
-      { iModIntro. iIntros. wp_apply ("IH" with "[] [$] [$]").
-        iPureIntro. by right. }
-      {
-        erewrite has_go_type_len.
-        2:{ eapply Helems. by left. }
-        rewrite right_id. setoid_rewrite Nat2Z.inj_add. setoid_rewrite <- loc_add_assoc.
-        iFrame.
-      }
-      iIntros "Hl".
-      wp_pures.
-      iApply "HΦ".
-      iFrame.
-      fold flatten_struct.
-      erewrite has_go_type_len.
-      2:{ eapply Helems. by left. }
-      rewrite right_id. setoid_rewrite Nat2Z.inj_add. setoid_rewrite <- loc_add_assoc.
-      by iFrame.
-    - (* case structT *)
-      rewrite struct.val_aux_unseal.
-      iInduction d as [|] "IH2" forall (l' Φ).
-      { wp_pures. iApply "HΦ". by iFrame. }
-      destruct a.
-      wp_pures.
-      iDestruct "Hl" as "[Hf Hl]".
-      fold flatten_struct.
-      wp_apply ("IH" with "[] Hf").
-      { iPureIntro. by left. }
-      iIntros "Hf".
-      replace (LitV (LitLoc l')) with (# l').
-      2:{ by rewrite to_val_unseal. }
-      wp_pures.
-      simpl.
-      wp_bind.
-      rewrite [in (to_val (l' +ₗ _))]to_val_unseal.
-      wp_apply ("IH2" with "[] [] [Hl]").
-      { iPureIntro. intros. apply Hfields. by right. }
-      { iModIntro. iIntros. wp_apply ("IH" with "[] [$] [$]").
-        iPureIntro. by right. }
-      {
-        erewrite has_go_type_len.
-        2:{ eapply Hfields. by left. }
-        rewrite right_id. setoid_rewrite Nat2Z.inj_add. setoid_rewrite <- loc_add_assoc.
-        iFrame.
-      }
-      iIntros "Hl".
-      wp_pures.
-      iApply "HΦ".
-      iFrame.
-      fold flatten_struct.
-      erewrite has_go_type_len.
-      2:{ eapply Hfields. by left. }
-      rewrite right_id. setoid_rewrite Nat2Z.inj_add. setoid_rewrite <- loc_add_assoc.
-      by iFrame.
-  Qed.
-
-  Lemma wp_store stk E l (v v' : val) :
-    {{{ ▷ heap_pointsto l (DfracOwn 1) v' }}} Store (Val $ LitV (LitLoc l)) (Val v) @ stk; E
-    {{{ RET LitV LitUnit; heap_pointsto l (DfracOwn 1) v }}}.
-  Proof.
-    iIntros (Φ) "Hl HΦ". wp_call.
-    wp_bind (PrepareWrite _).
-    iApply (wp_prepare_write with "Hl"); iNext; iIntros "[Hl Hl']".
-    wp_pures.
-    by iApply (wp_finish_store with "[$Hl $Hl']").
-  Qed.
-
-  Lemma wp_mem_store stk E l v v' :
-    {{{ ▷ l ↦ v }}}
-      (#l <-[t] #v')%V @ stk; E
-    {{{ RET #(); l ↦ v' }}}.
-  Proof using IntoValTyped0.
-    iIntros (Φ) ">Hl HΦ".
-    unseal.
-    pose proof (to_val_has_go_type v) as Hty_old.
-    pose proof (to_val_has_go_type v') as Hty.
-    generalize dependent #v. generalize dependent #v'.
-    clear dependent V. intros v' Hty v Hty_old.
-    iAssert (▷ (([∗ list] j↦vj ∈ flatten_struct v', heap_pointsto (l +ₗ j) (DfracOwn 1) vj) -∗ Φ #()))%I with "[HΦ]" as "HΦ".
-    { iIntros "!> HPost".
-      iApply "HΦ". iFrame. }
-    rename l into l'.
-    rewrite mem.store_unseal.
-    iInduction Hty_old as [] "IH" forall (v' Hty l' Φ) "HΦ".
-    all: inversion_clear Hty; subst;
-      try destruct i, i0; rewrite ?to_val_unseal /= ?loc_add_0 ?right_id; wp_pures.
-    all: try (wp_apply (wp_store with "[$]"); iIntros "H"; iApply "HΦ"; iFrame).
-    - (* array *)
-      rename a0 into a'.
-      iInduction a as [|] "IH2" forall (l' a' Helems0 Hlen0).
-      { simpl. wp_pures. rewrite ?to_val_unseal. iApply "HΦ".
-        dependent destruction a'; done. }
-      wp_pures.
-      iDestruct "Hl" as "[Hf Hl]".
-      fold flatten_struct.
-      erewrite has_go_type_len.
-      2:{ eapply Helems. by left. }
-      setoid_rewrite Nat2Z.inj_add. setoid_rewrite <- loc_add_assoc.
-      dependent destruction a'; first done.
-      simpl.
-      wp_pures.
-      wp_apply ("IH" with "[] [] [$Hf]").
-      { iPureIntro. simpl. by left. }
-      { iPureIntro. apply Helems0. by left. }
-      iIntros "Hf".
-      replace (LitV l') with (#l').
-      2:{ rewrite to_val_unseal //. }
-      wp_pures.
-      rewrite [in (to_val (l' +ₗ _))]to_val_unseal.
-      wp_apply ("IH2" with "[] [] [] [] [Hl]").
-      { iPureIntro. intros. apply Helems. by right. }
-      { iPureIntro. intros. apply Helems0. by right. }
-      { iPureIntro. simpl in *. lia. }
-      { iModIntro. iIntros. wp_apply ("IH" with "[] [//] [$] [$]"). iPureIntro. by right. }
-      { rewrite ?right_id. iFrame. }
-      iIntros "Hl".
-      iApply "HΦ".
-      iFrame.
-      fold flatten_struct.
-      erewrite has_go_type_len.
-      2:{ eapply Helems0. by left. }
-      setoid_rewrite Nat2Z.inj_add. setoid_rewrite <- loc_add_assoc.
-      rewrite ?right_id. iFrame.
-    - (* struct *)
-      rewrite struct.val_aux_unseal.
-      unfold struct.val_aux_def.
-      iInduction d as [|] "IH2" forall (l').
-      { wp_pures. rewrite to_val_unseal /=. iApply "HΦ". done. }
-      destruct a.
-      wp_pures.
-      iDestruct "Hl" as "[Hf Hl]".
-      fold flatten_struct.
-      erewrite has_go_type_len.
-      2:{ eapply Hfields. by left. }
-      setoid_rewrite Nat2Z.inj_add. setoid_rewrite <- loc_add_assoc.
-      wp_apply ("IH" with "[] [] [$Hf]").
-      { iPureIntro. simpl. by left. }
-      { iPureIntro. apply Hfields0. by left. }
-      iIntros "Hf".
-      replace (LitV l') with (#l').
-      2:{ rewrite to_val_unseal //. }
-      wp_pures.
-      rewrite [in (to_val (l' +ₗ _))]to_val_unseal.
-      wp_apply ("IH2" with "[] [] [] [Hl]").
-      { iPureIntro. intros. apply Hfields. by right. }
-      { iPureIntro. intros. apply Hfields0. by right. }
-      { iModIntro. iIntros. wp_apply ("IH" with "[] [//] [$] [$]"). iPureIntro. by right. }
-      { rewrite ?right_id. iFrame. }
-      iIntros "Hl".
-      iApply "HΦ".
-      iFrame.
-      fold flatten_struct.
-      erewrite has_go_type_len.
-      2:{ eapply Hfields0. by left. }
-      setoid_rewrite Nat2Z.inj_add. setoid_rewrite <- loc_add_assoc.
-      rewrite ?right_id. iFrame.
-  Qed.
-
-  Definition is_primitive_type (t : go_type) : Prop :=
-    match t with
-    | structT d => False
-    | arrayT n t => False
-    | funcT => False
-    | sliceT => False
-    | interfaceT => False
-    | _ => True
+  Ltac2 is_cmpxchg_inv () :=
+    match! goal with
+    | [ |- _ ] => progress subst
+    | [ h : is_cmpxchg_type _ _ |- _] =>
+        (Std.inversion Std.FullInversion (Std.ElimOnIdent h) None None;
+        Std.clear [h])
+    | [ h : existT _ _ = existT _ _ |- _ ] =>
+        Std.apply false false [(fun () => (constr:(Eqdep.EqdepTheory.inj_pair2), Std.ImplicitBindings []))]
+          (Some (h, None))
     end.
 
-  Lemma wp_typed_cmpxchg_fail s E l dq v' v1 v2 :
-    is_primitive_type t →
+  Ltac is_cmpxchg_inv := repeat ltac2:(is_cmpxchg_inv ()).
+
+  Lemma wp_typed_cmpxchg_fail `{!IntoVal V} `{!TypedPointsto V} t s E l dq (v' v1 v2 : V) :
+    is_cmpxchg_type t V →
     #v' ≠ #v1 →
-    {{{ ▷ l ↦{dq} v' }}} CmpXchg (Val # l) #v1 #v2 @ s; E
+    {{{ ▷ l ↦{dq} v' }}}
+      CmpXchg (Val # l) #v1 #v2 @ s; E
     {{{ RET (#v', #false); l ↦{dq} v' }}}.
   Proof using Type*.
-    pose proof (to_val_has_go_type v') as Hty_old.
-    pose proof (to_val_has_go_type v1) as Hty.
-    unseal.
-    generalize dependent (to_val v1). generalize dependent (to_val v'). generalize dependent (to_val v2).
-    intros.
-    clear dependent V.
-    rewrite to_val_unseal.
-    iIntros "Hl HΦ".
-    destruct t; try by exfalso.
-    all: inversion Hty_old; subst; inversion Hty; subst;
-      simpl; rewrite to_val_unseal /= in H0 |- *;
-      rewrite loc_add_0 right_id;
+    iIntros "%Hty %Hne % Hl HΦ". is_cmpxchg_inv.
+    all: rewrite typed_pointsto_unseal /=  into_val_unseal /= in Hne |- *;
       iApply (wp_cmpxchg_fail with "[$]"); first done; first (by econstructor);
-      iIntros; iApply "HΦ"; iFrame; done.
+      iFrame.
   Qed.
 
-  Lemma wp_typed_cmpxchg_suc s E l v' v1 v2 :
-    is_primitive_type t →
+  Lemma wp_typed_cmpxchg_suc `{!IntoVal V} `{!TypedPointsto V} t s E l (v' v1 v2 : V) :
+    is_cmpxchg_type t V →
     #v' = #v1 →
     {{{ ▷ l ↦ v' }}} CmpXchg #l #v1 #v2 @ s; E
     {{{ RET (#v', #true); l ↦ v2 }}}.
   Proof using Type*.
-    intros Hprim Heq.
-    pose proof (to_val_has_go_type v') as Hty_old.
-    pose proof (to_val_has_go_type v2) as Hty.
-    unseal.
-    generalize dependent (#v1). generalize dependent (#v'). generalize dependent (#v2).
-    clear dependent V.
-    intros.
-    iIntros "Hl HΦ".
-    destruct t; try by exfalso.
-    all: inversion Hty_old; subst;
-      inversion Hty; subst;
-      simpl; rewrite to_val_unseal /= loc_add_0 !right_id;
+    iIntros "%Hty %Hne % Hl HΦ". is_cmpxchg_inv.
+    all: rewrite typed_pointsto_unseal /=  into_val_unseal /= in Hne |- *;
       iApply (wp_cmpxchg_suc with "[$Hl]"); first done; first (by econstructor);
-      iIntros; iApply "HΦ"; iFrame; done.
+      iFrame.
   Qed.
 
-  Lemma wp_typed_Load s E (l : loc) (v : V) dq :
-    is_primitive_type t →
-    {{{ l ↦{dq} v }}}
+  Lemma wp_typed_Load s E `{!IntoVal V} `{!TypedPointsto V} t l dq (v : V) :
+    is_cmpxchg_type t V →
+    {{{ ▷ l ↦{dq} v }}}
       ! #l @ s ; E
     {{{ RET #v; l ↦{dq} v }}}.
   Proof using Type*.
-    intros Hprim.
-    pose proof (to_val_has_go_type v) as Hty.
-    unseal.
-    generalize dependent (#v).
-    clear dependent V.
-    intros.
-    iIntros "Hl HΦ".
-    destruct t; try by exfalso.
-    all: inversion Hty; subst;
-      inversion Hty; subst;
-      simpl; rewrite to_val_unseal /= loc_add_0 !right_id;
-      iApply (wp_load with "[$Hl]"); iFrame.
+    intros Hty. is_cmpxchg_inv.
+    all: rewrite typed_pointsto_unseal /=  into_val_unseal /=; eapply lifting.wp_load.
   Qed.
 
-  Lemma wp_typed_AtomicStore s E (l : loc) (v v' : V) :
-    is_primitive_type t →
-    {{{ l ↦ v }}}
+  Lemma wp_typed_AtomicStore s E `{!IntoVal V} `{!TypedPointsto V} t l (v v' : V) :
+    is_cmpxchg_type t V →
+    {{{ ▷ l ↦ v }}}
       AtomicStore #l #v' @ s ; E
     {{{ RET #(); l ↦ v' }}}.
   Proof using Type*.
-    intros Hprim.
-    pose proof (to_val_has_go_type v) as Hty_old.
-    pose proof (to_val_has_go_type v') as Hty.
-    unseal.
-    generalize dependent (#v). generalize dependent (#v').
-    clear dependent V.
-    intros.
-    iIntros "Hl HΦ".
-    destruct t; try by exfalso.
-    all: inversion Hty; subst;
-      inversion Hty_old; inversion Hty; subst;
-      simpl; rewrite to_val_unseal /= loc_add_0 !right_id;
-      iApply (wp_atomic_store with "[$Hl]"); iFrame.
+    intros Hty. is_cmpxchg_inv.
+    all: rewrite typed_pointsto_unseal /=  into_val_unseal /=; eapply wp_atomic_store.
   Qed.
 
 End goose_lang.
 
-Notation "l ↦ dq v" := (typed_pointsto l dq v%V)
-                              (at level 20, dq custom dfrac at level 50,
-                               format "l  ↦ dq  v") : bi_scope.
-
 Section tac_lemmas.
   Context `{ffi_sem: ffi_semantics} `{!ffi_interp ffi} `{!heapGS Σ}.
 
-  Class PointsToAccess {V} {t} `{!IntoVal V} `{!IntoValTyped V t}
+  Class PointsToAccess {V} `{!IntoVal V} `{!TypedPointsto V}
     (l : loc) (v : V) dq (P : iProp Σ) (P' : V → iProp Σ) : Prop :=
     {
       points_to_acc : P -∗ l ↦{dq} v ∗ (∀ v', l ↦{dq} v' -∗ P' v');
       points_to_update_eq : P' v ⊣⊢ P;
     }.
 
-  Global Instance points_to_access_trivial {V} l (v : V) {t} `{!IntoVal V} `{!IntoValTyped V t} dq
+  Global Instance points_to_access_trivial {V} l (v : V) `{!IntoVal V} `{!TypedPointsto V} dq
     : PointsToAccess l v dq (l ↦{dq} v)%I (λ v', l ↦{dq} v')%I.
   Proof. constructor; [eauto with iFrame|done]. Qed.
 
-  Lemma tac_wp_load {V t} `{!IntoVal V} `{!IntoValTyped V t}
+  Lemma tac_wp_load {V t} `{!IntoVal V} `{!TypedPointsto V} `{!IntoValTyped V t}
     K (l : loc) (v : V) Δ s E i dq Φ is_pers
     `{!PointsToAccess l v dq P P'} :
     envs_lookup i Δ = Some (is_pers, P)%I →
     envs_entails Δ (WP (fill K (Val #v)) @ s; E {{ Φ }}) →
-    envs_entails Δ (WP (fill K (mem.load t #l)) @ s; E {{ Φ }}).
+    envs_entails Δ (WP (fill K (load t #l)) @ s; E {{ Φ }}).
   Proof using Type*.
     rewrite envs_entails_unseal => ? HΦ.
     rewrite envs_lookup_split //.
@@ -605,40 +111,36 @@ Section tac_lemmas.
     destruct is_pers; simpl.
     - iDestruct "H" as "#H".
       iDestruct (points_to_acc with "H") as "[H' _]".
-      unshelve wp_apply (wp_mem_load with "[$]"); first apply _.
-      iIntros "?".
+      wp_apply (wp_load with "[$]"). iIntros "?".
       iApply HΦ. iApply "Henv". iFrame "#".
     - iDestruct (points_to_acc with "H") as "[H Hclose]".
-      unshelve wp_apply (wp_mem_load with "[$]"); first apply _.
-      iIntros "?".
+      wp_apply (wp_load with "[$]"). iIntros "?".
       iApply HΦ. iApply "Henv".
       iSpecialize ("Hclose" with "[$]").
       rewrite points_to_update_eq. iFrame.
   Qed.
 
-  Lemma tac_wp_store {V t} `{!IntoVal V} `{!IntoValTyped V t}
+  Lemma tac_wp_store {V t} `{!IntoVal V} `{!TypedPointsto V} `{!IntoValTyped V t}
     K (l : loc) (v v' : V) Δ Δ' s E i Φ
     `{!PointsToAccess l v (DfracOwn 1) P P'} :
     envs_lookup i Δ = Some (false, P)%I →
     envs_simple_replace i false (Esnoc Enil i (P' v')) Δ = Some Δ' →
     envs_entails Δ' (WP fill K (Val #()) @ s ; E {{ Φ }}) →
-    envs_entails Δ (WP (fill K (mem.store t #l (Val #v'))) @ s; E {{ Φ }}).
+    envs_entails Δ (WP (fill K (store t #l (Val #v'))) @ s; E {{ Φ }}).
   Proof.
     rewrite envs_entails_unseal => ?? HΦ.
     rewrite envs_simple_replace_sound // /=.
     iIntros "[H Henv]".
     iDestruct (points_to_acc with "H") as "[H Hclose]".
-    unshelve wp_apply (wp_mem_store with "[$]"); first tc_solve.
-    iIntros "H". iSpecialize ("Hclose" with "[$]").
-    iApply HΦ.
+    wp_apply (wp_store with "[$]"). iIntros "H".
+    iSpecialize ("Hclose" with "[$]"). iApply HΦ.
     iApply "Henv". iFrame.
   Qed.
 
   Lemma tac_wp_alloc
-    `{!IntoVal V} `{!IntoValTyped V t}
-    K Δ stk E Φ :
-    (∀ l, envs_entails Δ (l ↦ (default_val V) -∗ WP (fill K (Val #l)) @ stk; E {{ Φ }})) →
-    envs_entails Δ (WP fill K (mem.alloc t #()) @ stk; E {{ Φ }}).
+    `{!IntoVal V} `{!TypedPointsto V} `{!IntoValTyped V t} K Δ stk E Φ :
+    (∀ l, envs_entails Δ (l ↦ (zero_val V) -∗ WP (fill K (Val #l)) @ stk; E {{ Φ }})) →
+    envs_entails Δ (WP fill K (alloc t #()) @ stk; E {{ Φ }}).
   Proof.
     rewrite envs_entails_unseal => Hwp.
     iIntros "Henv".
@@ -653,7 +155,7 @@ Ltac2 tc_solve_many () := solve [ltac1:(typeclasses eauto)].
 Ltac2 ectx_simpl () := cbv [fill flip foldl ectxi_language.fill_item goose_ectxi_lang fill_item].
 
 Ltac2 wp_load_visit e k :=
-  Control.once_plus (fun () => Std.unify e '(mem.load _ (Val _)))
+  Control.once_plus (fun () => Std.unify e '(load _ (Val _)))
          (fun _ => Control.zero Walk_expr_more);
   Control.once_plus (fun _ => eapply (tac_wp_load $k) > [tc_solve_many ()| ltac1:(iAssumptionCore) | ectx_simpl ()])
     (fun _ => Control.backtrack_tactic_failure "wp_load: could not find a points-to in context covering the address")
@@ -667,7 +169,7 @@ Ltac2 wp_load () :=
   end.
 
 Ltac2 wp_store_visit e k :=
-  Control.once_plus (fun () => (Std.unify e '(mem.store _ _ (Val _))))
+  Control.once_plus (fun () => (Std.unify e '(store _ _ (Val _))))
          (fun _ => Control.zero Walk_expr_more);
   Control.once_plus (fun _ => eapply (tac_wp_store $k) > [tc_solve_many ()| ltac1:(iAssumptionCore)
                                            |ltac1:(pm_reflexivity) | ectx_simpl () ])
@@ -682,7 +184,7 @@ Ltac2 wp_store () :=
   end.
 
 Ltac2 wp_alloc_visit e k :=
-  Control.once_plus (fun () => Std.unify e '(mem.alloc _ #()))
+  Control.once_plus (fun () => Std.unify e '(alloc _ #()))
     (fun _ => Control.zero Walk_expr_more);
   Control.once_plus (fun _ => eapply (tac_wp_alloc $k); ectx_simpl ())
     (fun _ => Control.backtrack_tactic_failure "wp_alloc: failed to apply tac_wp_alloc")
@@ -699,7 +201,7 @@ Ltac2 wp_alloc_auto_visit e k :=
   lazy_match! e with
   (* Manually writing out [let: ?var_name := (ref_ty _ (Val _)) in ?e1] to get
      pattern matching to work. *)
-  | (App (Rec BAnon (BNamed ?var_name) ?e1) (App (Val (mem.alloc _)) (Val #()))) =>
+  | (App (Rec BAnon (BNamed ?var_name) ?e1) (App (Val (alloc _)) (Val #()))) =>
       let let_expr1 := '(Rec BAnon (BNamed $var_name) $e1) in
       let ptr_name := Std.eval_vm None constr:($var_name +:+ "_ptr") in
       let k := constr:(@AppRCtx _ $let_expr1 :: $k) in
