new/golang/defn/postlang.v
@@ -20,6 +20,22 @@ Notation "e1 || e2" :=
 Global Notation "# x" := (into_val x%go).
 Global Notation "#" := into_val (at level 0).
 
+(* built-in functions *)
+Definition make3 : go_string := "make3".
+Definition make2 : go_string := "make2".
+Definition make1 : go_string := "make1".
+Definition len : go_string := "len".
+Definition cap : go_string := "cap".
+
+(* helpers for signed comparisons *)
+Section helpers.
+Context `{ffi_syntax}.
+Definition int_lt : val := λ: "x" "y", BinOp SignedLtOp "x" "y".
+Definition int_leq : val := λ: "x" "y", BinOp SignedLeOp "x" "y".
+Definition int_geq : val := λ: "x" "y", int_leq "y" "x".
+Definition int_gt : val := λ: "x" "y", int_lt "y" "x".
+End helpers.
+
 Module go.
 
 (* built-in types *)
@@ -36,32 +52,20 @@ Definition bool : go.type := go.Named "bool"%go [].
 Definition byte : go.type := uint8.
 Definition rune : go.type := uint32.
 
-(* built-in functions *)
-Definition make3 : go_string := "make3".
-Definition make2 : go_string := "make2".
-Definition len : go_string := "len".
-Definition cap : go_string := "cap".
-
 Section defs.
 Context `{ffi_syntax}.
 
-(* helpers for signed comparisons *)
-Definition int_lt : val := λ: "x" "y", BinOp SignedLtOp "x" "y".
-Definition int_leq : val := λ: "x" "y", BinOp SignedLeOp "x" "y".
-Definition int_geq : val := λ: "x" "y", int_leq "y" "x".
-Definition int_gt : val := λ: "x" "y", int_lt "y" "x".
-
 Inductive is_primitive : go.type → Prop :=
-| is_primitive_uint64 : is_primitive uint64
-| is_primitive_uint32 : is_primitive uint32
-| is_primitive_uint16 : is_primitive uint16
-| is_primitive_uint8 : is_primitive uint8
-| is_primitive_int64 : is_primitive int64
-| is_primitive_int32 : is_primitive int32
-| is_primitive_int16 : is_primitive int16
-| is_primitive_int8 : is_primitive int8
-| is_primitive_string : is_primitive string
-| is_primitive_bool : is_primitive bool
+| is_primitive_uint64 : is_primitive go.uint64
+| is_primitive_uint32 : is_primitive go.uint32
+| is_primitive_uint16 : is_primitive go.uint16
+| is_primitive_uint8 : is_primitive go.uint8
+| is_primitive_int64 : is_primitive go.int64
+| is_primitive_int32 : is_primitive go.int32
+| is_primitive_int16 : is_primitive go.int16
+| is_primitive_int8 : is_primitive go.int8
+| is_primitive_string : is_primitive go.string
+| is_primitive_bool : is_primitive go.bool
 
 | is_primitive_pointer t : is_primitive (go.PointerType t)
 | is_primitive_function sig : is_primitive (go.FunctionType sig)
@@ -71,14 +75,14 @@ Inductive is_primitive : go.type → Prop :=
 | is_primitive_channel dir t : is_primitive (go.ChannelType dir t).
 
 Inductive is_primitive_zero_val : go.type → ∀ {V} `{!IntoVal V}, V → Prop :=
-| is_primitive_zero_val_uint64 : is_primitive_zero_val uint64 (W64 0)
-| is_primitive_zero_val_uint32 : is_primitive_zero_val uint32 (W32 0)
-| is_primitive_zero_val_uint16 : is_primitive_zero_val uint16 (W16 0)
-| is_primitive_zero_val_uint8 : is_primitive_zero_val uint8 (W8 0)
-| is_primitive_zero_val_int64 : is_primitive_zero_val int64 (W64 0)
-| is_primitive_zero_val_int32 : is_primitive_zero_val int32 (W32 0)
-| is_primitive_zero_val_int16 : is_primitive_zero_val int16 (W16 0)
-| is_primitive_zero_val_int8 : is_primitive_zero_val int8 (W8 0)
+| is_primitive_zero_val_uint64 : is_primitive_zero_val go.uint64 (W64 0)
+| is_primitive_zero_val_uint32 : is_primitive_zero_val go.uint32 (W32 0)
+| is_primitive_zero_val_uint16 : is_primitive_zero_val go.uint16 (W16 0)
+| is_primitive_zero_val_uint8 : is_primitive_zero_val go.uint8 (W8 0)
+| is_primitive_zero_val_int64 : is_primitive_zero_val go.int64 (W64 0)
+| is_primitive_zero_val_int32 : is_primitive_zero_val go.int32 (W32 0)
+| is_primitive_zero_val_int16 : is_primitive_zero_val go.int16 (W16 0)
+| is_primitive_zero_val_int8 : is_primitive_zero_val go.int8 (W8 0)
 | is_primitive_zero_val_string : is_primitive_zero_val go.string ""%go
 | is_primitive_zero_val_bool : is_primitive_zero_val go.bool false
 
@@ -90,9 +94,9 @@ Inductive is_primitive_zero_val : go.type → ∀ {V} `{!IntoVal V}, V → Prop 
 | is_primitive_zero_val_channel dir t : is_primitive_zero_val (go.ChannelType dir t) null
 .
 
-(** [go.ValidCore] defines when a GoContext is valid, excluding map, and channel
-    stuff. *)
-Class ValidCore `{!GoContext} :=
+(** [go.ValidCore] defines when a GoContext is valid, excluding slice, map, and
+    channel stuff. *)
+Class CoreSemantics `{!GoContext} :=
 {
   alloc_underlying t : alloc t = alloc (to_underlying t);
   alloc_primitive t {V} (v : V) `{!IntoVal V} (H : is_primitive_zero_val t v) :
@@ -178,43 +182,22 @@ Class ValidCore `{!GoContext} :=
   index_ref_underlying t : index_ref t = index_ref (to_underlying t);
   index_ref_array n elem_type i l :
     index_ref (go.ArrayType n elem_type) i #l = #(array_index_ref elem_type i l);
-  index_ref_slice elem_type i s (Hrange : 0 ≤ i < sint.Z s.(slice.len)) :
-    index_ref (go.SliceType elem_type) i #s = #(slice_index_ref elem_type i s);
 
   index_underlying t : index t = index (to_underlying t);
   index_array n elem_type i l v (Hinrange : l !! (Z.to_nat i) = Some v):
     index (go.ArrayType n elem_type) i (ArrayV l) = (Val v);
-  index_slice elem_type i (s : slice.t) :
-    index (go.SliceType elem_type) i #s =
-    GoInstruction (GoLoad elem_type) $ GoInstruction (Index $ go.SliceType elem_type) #(W64 i) #s;
 
   len_underlying t : functions len [t] = functions len [to_underlying t];
-  len_slice elem_type :
-    functions len [go.TypeLit $ go.SliceType elem_type] =
-    (λ: "s", GoInstruction (InternalLen (go.SliceType elem_type)) "s")%V;
 
   cap_underlying t : functions cap [t] = functions cap [to_underlying t];
-  cap_slice elem_type :
-      functions cap [go.TypeLit $ go.SliceType elem_type] =
-      (λ: "s", GoInstruction (InternalCap (go.SliceType elem_type)) "s")%V;
 
   make3_underlying t : functions make3 [t] = functions make3 [to_underlying t];
-  make3_slice elem_type :
-    functions make3 [go.TypeLit $ go.SliceType elem_type] =
-    (λ: "t" "len" "cap",
-       if: (int_lt "cap" "len") then Panic "makeslice: cap out of range" else #();;
-       if: (int_lt "len" #(W64 0)) then Panic "makeslice: len out of range" else #();;
-       if: "cap" = #(W64 0) then
-         (* XXX: this computes a nondeterministic unallocated address by using
-            "(Loc 1 0) +ₗ ArbiraryInt"*)
-         GoInstruction InternalMakeSlice (#(Loc 1 0) +ₗ ArbitraryInt, "len", "cap")
-       else
-         let: "p" := GoInstruction (InternalDynamicArrayAlloc elem_type) "cap" in
-         GoInstruction InternalMakeSlice ("p", "len", "cap"))%V;
-  make2_unfold t :
-    functions make2 [t] =
-    (λ: "t" "sz", GoInstruction (FuncCall make3 [t]) #() "t" "sz" "sz")%V;
+  make2_underlying t : functions make2 [t] = functions make2 [to_underlying t];
+  make1_underlying t : functions make1 [t] = functions make1 [to_underlying t];
 }.
 
 End defs.
 End go.
+
+Global Notation func_call := (GoInstruction FuncCall).
+Global Notation method_call := (GoInstruction MethodCall).
